certicoq/theories/Extraction/extraction.v
@@ -23,10 +23,6 @@ Require Import ExtrOcamlString.
 Extract Inlined Constant Coqlib.proj_sumbool => "(fun x -> x)".
 
 
-(* L5_to_L6 *)
-Extract Constant L5_to_L6.fun_tag => "Camlcoq.P.of_int 3".
-Extract Constant L5_to_L6.kon_tag => "Camlcoq.P.of_int 2".
-Extract Constant L5_to_L6.default_tag => "Camlcoq.P.of_int 1".
 (* L6_to_Clight *)
 Extract Constant L6_to_Clight.print_Clight => "PrintClight.print_if".
 Extract Constant L6_to_Clight.print_Clight_dest => "PrintClight.print_dest".
